proof/refine/PageTableDuplicates.thy
@@ -2041,9 +2041,9 @@ crunch valid_duplicates'[wp]:
 lemma invokeIRQControl_valid_duplicates'[wp]:
   "\<lbrace>\<lambda>s. vs_valid_duplicates' (ksPSpace s) \<rbrace> invokeIRQControl a
   \<lbrace>\<lambda>_ s. vs_valid_duplicates' (ksPSpace s)\<rbrace>"
-  apply (simp add:invokeIRQControl_def invokeInterruptControl_def)
+  apply (simp add:invokeIRQControl_def ArchInterrupt_H.invokeIRQControl_def)
   apply (rule hoare_pre)
-  apply (wp|wpc | simp add:invokeInterruptControl_def)+
+  apply (wp|wpc | simp add:ArchInterrupt_H.invokeIRQControl_def)+
   apply fastforce
  done
 
@@ -2052,7 +2052,7 @@ lemma invokeIRQHandler_valid_duplicates'[wp]:
   \<lbrace>\<lambda>_ s. vs_valid_duplicates' (ksPSpace s)\<rbrace>"
   apply (simp add:invokeIRQHandler_def)
   apply (rule hoare_pre)
-  apply (wp|wpc | simp add:invokeInterruptControl_def)+
+  apply (wp|wpc | simp add: ArchInterrupt_H.invokeIRQControl_def)+
   done
 
 lemma invokeCNode_valid_duplicates'[wp]:
